@prefix : <http://www.researchspace.org/resource/> .
@prefix rs: <http://www.researchspace.org/ontology/> .
@prefix User: <http://www.researchspace.org/resource/user/> .
@prefix Help: <http://help.researchspace.org/resource/> .
@prefix Platform: <http://www.researchspace.org/resource/system/> .
@prefix owl: <http://www.w3.org/2002/07/owl#> .
@prefix xsd: <http://www.w3.org/2001/XMLSchema#> .
@prefix skos: <http://www.w3.org/2004/02/skos/core#> .
@prefix rdfs: <http://www.w3.org/2000/01/rdf-schema#> .
@prefix crmdig: <http://www.ics.forth.gr/isl/CRMdig/> .
@prefix rshelp: <http://researchspace.org/help/> .
@prefix crmsci: <http://www.ics.forth.gr/isl/CRMsci/> .
@prefix crmgeo: <http://www.ics.forth.gr/isl/CRMgeo/> .
@prefix sp: <http://spinrdf.org/sp#> .
@prefix prov: <http://www.w3.org/ns/prov#> .
@prefix crminfluence: <http://www.cidoc-crm.org/cidoc-crm/influence/> .
@prefix crm: <http://www.cidoc-crm.org/cidoc-crm/> .
@prefix crminf: <http://www.ics.forth.gr/isl/CRMinf/> .
@prefix Admin: <http://www.researchspace.org/resource/admin/> .
@prefix bds: <http://www.bigdata.com/rdf/search#> .
@prefix rdf: <http://www.w3.org/1999/02/22-rdf-syntax-ns#> .
@prefix crmba: <http://www.cidoc-crm.org/cidoc-crm/CRMba/> .
@prefix ontodia: <http://ontodia.org/schema/v1#> .
@prefix crmarchaeo: <http://www.cidoc-crm.org/cidoc-crm/CRMarchaeo/> .
@prefix forms: <http://www.researchspace.org/resource/system/forms/> .
@prefix frbroo: <http://iflastandards.info/ns/fr/frbr/frbroo/> .

<http://www.researchspace.org/ontology/context> {

  <http://www.researchspace.org/ontology/> a <http://www.w3.org/ns/ldp#Resource>, prov:Entity,
      owl:Ontology;
    rdfs:label "ResearchSpace ontology"@en ;
    prov:generatedAtTime "2021-10-04T05:27:54.915Z"^^xsd:dateTime;
    prov:wasAttributedTo User:admin .

     <http://www.researchspace.org/resource/system/ontologyContainer> <http://www.w3.org/ns/ldp#contains>
    <http://www.researchspace.org/ontology/> .

  rs:EX_Association a owl:Class;
    rdfs:label "Association";
    rdfs:comment "This is a specialisation of Attribute Assignment in order to assign attributes and typing of properties which are sub properties / specialisations of CRM asserted in the British Museum ontology";
    rdfs:subClassOf crm:E13_Attribute_Assignment .
  
  rs:PX_field_of_activity_of_the_agent a owl:DatatypeProperty;
    rdfs:subPropertyOf crm:P3_has_note;
    rdfs:seeAlso "http://rdvocab.info/ElementsGr2/fieldOfActivityOfTheCorporateBody";
    rdfs:label "field of activity of agent";
    rdfs:comment "This is similar to RDA Group 2 Elements properties 'Field of acttivity of the corporate body' and 'Field of acttivity of person' but instead allows just the agent to be expressed as BM bio records do not accurately distinguish between individuals & institutions." .
  
  rs:PX_exhibition_history a owl:DatatypeProperty;
    rdfs:label "exhibition history";
    rdfs:subPropertyOf crm:P3_has_note;
    rdfs:comment "This is a sub-property of crm:P3_has_note, used to represent the exhibition history of an object" .
  
  rs:EX_Digital_Image_Region a owl:Class;
    rdfs:label "Digitial Image Region";
    rdfs:comment "Image regions are the direct result of a digital machine event on an digital image according to CRMdig.";
    rdfs:subClassOf crmdig:D9_Data_Object .
  
  rs:PX_display_wrap a owl:DatatypeProperty;
    rdfs:label "display wrap";
    rdfs:comment "This predicate is to encapsulate text/notes which are for indexing and to explain in a text format structured data represented in RDF";
    rdfs:subPropertyOf crm:P3_has_note .
  
  rs:PX_has_main_representation a owl:ObjectProperty;
    rdfs:subPropertyOf crm:P138i_has_representation;
    rdfs:label "has main representation";
    rdfs:range crm:E38_Image;
    rdfs:comment "This is to identifier the primary representation an object may have";
    rdfs:domain crm:E22_Man-Made_Object;
    owl:inverseOf rs:PX_main_represents .
  
  rs:PX_currency a owl:ObjectProperty;
    rdfs:label "currency";
    rdfs:subPropertyOf crm:P2_has_type .
  
  rs:EX_Bibliographic_Series a owl:Class;
    rdfs:subClassOf crm:E89_Propositional_Object;
    rdfs:label "Bibliographic Series";
    rdfs:comment "This is a specific series which can comprise of many different documents which belong together as a specific series collection" .
  
  rs:PX_condition a owl:DatatypeProperty;
    rdfs:label "condition";
    rdfs:subPropertyOf crm:P3_has_note .
  
  rs:displayLabel a owl:DatatypeProperty;
    rdfs:comment ""@en;
    rdfs:range xsd:string;
    rdfs:label "display label"@en .
  
  rs:PX_has_transliteration a owl:DatatypeProperty;
    rdfs:subPropertyOf crm:P3_has_note;
    rdfs:label "has transliteration";
    rdfs:comment "This is a sub-property of crm:P3_has_note, used to represent a transliteration of an inscription" .
  
  rs:PX_gender a owl:ObjectProperty;
    rdfs:label "gender";
    rdfs:subPropertyOf crm:P2_has_type .
  
  rs:EX_Digital_Image a owl:Class;
    rdfs:comment "Digital images are both CRM images and digital objects according to CRMdig.";
    rdfs:subClassOf crm:E38_Image, crmdig:D1_Digital_Object;
    rdfs:label "Digital Image" .
  
  rs:PX_curatorial_comment a owl:DatatypeProperty;
    rdfs:subPropertyOf crm:P3_has_note;
    rdfs:label "curatorial comment" .
  
  rs:PX_escapement a owl:ObjectProperty;
    rdfs:subPropertyOf crm:P2_has_type;
    rdfs:label "escapement" .
  
  rs:FieldInstance a owl:Class;
    rdfs:label "Field" .
  
  rs:EX_Discovery a owl:Class;
    rdfs:comment "This is a subclass of E7_Activity which describes the event at which a persistent item was found.";
    rdfs:subClassOf crm:E7_Activity;
    rdfs:label "Discovery" .
  
  rs:PX_inscription_position a owl:DatatypeProperty;
    rdfs:subPropertyOf crm:P3_has_note;
    rdfs:comment "This is an extension of has_note for the free text field in BM collections system \"Inscription Position\"";
    rdfs:label "inscription position" .
  
  rs:EX_Repair a owl:Class;
    rdfs:subClassOf crm:E11_Modification;
    rdfs:comment "This is a sub-class of crm:E11.Modification, used to represent an activity which involves the repair of an object";
    rdfs:label "Repair" .
  
  rs:EX_Assertion a owl:Class;
    rdfs:label "Assertion";
    rdfs:subClassOf crm:E7_Activity;
    rdfs:comment "Records the beliefs asserted into the system by a given user" .
  
  rs:PX_commemorates a owl:ObjectProperty;
    rdfs:subPropertyOf crm:P67_refers_to;
    rdfs:label "commemorates" .
  
  rs:PX_inscription_script a owl:ObjectProperty;
    rdfs:comment "This is a sub-property of crm:P2_has_type, This predicate is used to identify the type of script in which an inscription is written (eg Roman, Hieroglyphic, etc)";
    rdfs:label "inscription script";
    rdfs:subPropertyOf crm:P2_has_type .
  
  rs:PX_main_represents a owl:ObjectProperty;
    rdfs:label "is main represetation of";
    owl:inverseOf rs:PX_has_main_representation;
    rdfs:subPropertyOf crm:P138_represents;
    rdfs:domain crm:E38_Image;
    rdfs:range crm:E22_Man-Made_Object;
    rdfs:comment "This is to identifier the primary representation of an object" .
  
  rs:PX_has_copyright a owl:DatatypeProperty;
    rdfs:comment "This is a sub-property of crm:P3_has_note, used to represent copyright information";
    rdfs:label "has copyright";
    rdfs:subPropertyOf crm:P3_has_note .
  
  rs:PX_asserts rdfs:domain rs:EX_Assertion;
    rdfs:range crminf:I2_Belief;
    rdfs:label "asserts";
    rdfs:type owl:ObjectProperty .
  
  rs:PX_type_series a owl:ObjectProperty;
    rdfs:label "type series";
    rdfs:subPropertyOf crm:P2_has_type .
  
  rs:PX_min_value a owl:DatatypeProperty;
    rdfs:label "min value";
    rdfs:subPropertyOf crm:P90_has_value;
    rdfs:comment "This is a sub-property of crm:P90_has_value, used to represent the either the value of a dimension, or the lower bound if the dimension is a range (in which case PX_max_value will also be specified)" .
  
  rs:PX_nationality a owl:ObjectProperty;
    rdfs:label "nationality";
    rdfs:subPropertyOf crm:P107i_is_current_or_former_member_of;
    rdfs:comment "This is the nationality of an E39 Actor.  It is a sub-property of P107i (is current or former member of) - thus the Nation is modelled as a group (E74)";
    rdfs:range crm:E74_Group;
    rdfs:domain crm:E39_Actor .
  
  rs:PX_object_exhibition_label a owl:DatatypeProperty;
    rdfs:label "object exhibition label";
    rdfs:subPropertyOf crm:P3_has_note .
  
  rs:PX_inscription_type a owl:ObjectProperty;
    rdfs:subPropertyOf crm:P2_has_type;
    rdfs:comment "This should be used with the thesauri/inscription thesauri";
    rdfs:label "inscription type" .
  
  rs:PX_likelihood a owl:ObjectProperty;
    rdfs:comment "BM Likelihood";
    rdfs:label "likelihood";
    rdfs:subPropertyOf crm:P2_has_type .
  
  rs:PX_physical_description a owl:DatatypeProperty;
    rdfs:label "physical exhibition";
    rdfs:subPropertyOf crm:P3_has_note;
    rdfs:comment "This is a sub-property of crm:P3_has_note, used to represent a physical description of an object" .
  
  rs:PX_stratigraphic_note a owl:DatatypeProperty;
    rdfs:label "stratigraphic note";
    rdfs:subPropertyOf crm:P3_has_note .
  
  rs:PX_pupil_of a owl:ObjectProperty;
    rdfs:label "Pupil of";
    rdfs:domain crm:E21_Person;
    rdfs:comment "This should be considered a shortcut for a CRM teaching activity";
    rdfs:range crm:E39_Actor .
  
  rs:PX_property a owl:ObjectProperty;
    rdfs:label "property";
    rdfs:domain rs:EX_Association;
    rdfs:comment "This is to be used with EX_Association in order to assign attributes to subproperties of CRM asserted in the British Museum Ontology" .
  
  rs:PX_profession a owl:ObjectProperty;
    rdfs:label "profession";
    rdfs:subPropertyOf crm:P107i_is_current_or_former_member_of;
    rdfs:range crm:E74_Group;
    rdfs:comment "This is the profession of an E39 Actor.  It is a sub-property of P107i (is current or former member of) - thus the profession is modelled as a group (E74)";
    rdfs:domain crm:E39_Actor .
  
  rs:targetsEntity a owl:ObjectProperty;
    rdfs:comment ""@en;
    rdfs:domain crminf:I1_Argumentation;
    rdfs:label "targets entity"@en;
    rdfs:range crm:E1_CRM_Entity .
  
  rs:PX_max_value a owl:DatatypeProperty;
    rdfs:comment "This is a sub-property of crm:P90_has_value, used to represent the maximum value of a dimension, where the dimension is a range (in which case PX_min_value will also be specified)";
    rdfs:label "max value";
    rdfs:subPropertyOf crm:P90_has_value .
  
  rs:PX_object_type a owl:ObjectProperty;
    rdfs:label "object type";
    rdfs:subPropertyOf crm:P2_has_type .
  
  rs:PX_inscription_subject a owl:ObjectProperty;
    rdfs:subPropertyOf crm:P2_has_type;
    rdfs:comment "This should be used with the id/thesauri/inscription-subject thesaurus";
    rdfs:label "inscription subject" .
  
  rs:targetsField a owl:ObjectProperty;
    rdfs:comment ""@en;
    rdfs:label "targets field"@en;
    rdfs:domain crminf:I1_Argumentation .
  
  rs:PX_ware a owl:ObjectProperty;
    rdfs:subPropertyOf crm:P2_has_type;
    rdfs:label "ware" .
}
